stuck in defining [timedEnv]

train.v
@@ -1,55 +1,43 @@
 
 Add LoadPath "../../../ssrcorn" as CoRN.
 Add LoadPath "../../../ssrcorn/math-classes/src" as MathClasses.
+Require Export ROSCyberPhysicalSystem.
+Require Export String.
 
-Require Export Process.
+Instance stringdeceqdsjfklsajlk : DecEq string.
+constructor. exact string_dec.
+Defined.
 
+Open Scope string_scope.
 
-Add LoadPath "../../../ssrcorn" as CoRN.
-Add LoadPath "../../../ssrcorn/math-classes/src" as MathClasses.
+Inductive Void :=.
 
-(** this is a 1D train between 2 stations
-    It has sensors on each side to estimate
-    the distance from endpoints.
-    The operator directly controls the velocity
-    of the train. In ideal world, he/she
-    controls the acceleration *)
-
-Record TrainState :=
-{
-  posX : R; (* this should really be R *)
-  vX : Q
-}.
-
-Open Scope Q_scope.
-
-Definition VelExactly  (vel : Q) : OutDevBehaviour R :=
-Build_OutDevBehaviour (fun tm rint =>  (forall t, rint t = Q2R vel)).
-
-Definition VelOutDevice : 
-  MemoryLessOutDev R Q :=
-  (VelExactly 0, fun q => VelExactly q).
+(** When adding a nrew topic, add cases of this function *)
+Definition stringTopic2Type (s : string) : Type :=
+if (eqdec s "motorRecv") then Q else
+if (eqdec s "timerSend") then unit else Void.
 
 
-(* MOVE !! *)
+Instance  ttttt : @RosTopicType string _.
+constructor. exact stringTopic2Type.
+Defined.
 
-Require Export model.structures.Qpossec.
+Inductive RosLoc := baseMotor | timerNode | digiController.
 
-Lemma mkTime (qp : Qpos) : Time.
-Admitted.
+Scheme Equality for RosLoc.
 
-
-(** outputs a message every [delay] seconds *)
-Definition Timer (delay : Qpos) : InpDev unit unit.
-cofix.
-  constructor. right.
-  split.
-  - split; [constructor|].
-    exact (mkTime delay). 
-  - exact Timer.
+Instance rldeqdsjfklsajlk : DecEq RosLoc.
+constructor. exact RosLoc_eq_dec.
 Defined.
 
 
-(** To model randomness, the device can
-  take a stream of random bits as input 
-  This randomness source can be a part of the environment.*)
+
+Instance rllllfjkfhsdakfsdakh : RosLocType RosLoc.
+(* we can't define the [timeValuedEnv]  component because
+   it is only function of the RosLoc, which does not have enough information.
+   One could add (Time -> R) to some nodes in RosLoc, but that
+   will give us infinitely many nodes, and also make equality undecidable.
+   [timeValuedEnv] is also a function of environment
+ *)
+
+
